Logic/Interpretability/PAHF/Coq/Audit.v
@@ -217,6 +217,10 @@ Check PA.Formula.betaCodingStepExistsTermAtBody.
 Check PA.Formula.betaPrependCodingStepTermAt.
 Check PA.Formula.betaPrependCodingStepExistsTermAt.
 Check PA.Formula.betaPrependCodingStepExistsTermAtBody.
+Check PA.Formula.betaUnshiftPrefixTermAt.
+Check PA.Formula.betaPrependPrefixTermAt.
+Check PA.Formula.betaPrependPrefixCodeExistsTermAt.
+Check PA.Formula.betaPrependPrefixCodeExistsTermAtBody.
 Check PA.Formula.subst_positiveCommonMultipleThroughTermAt.
 Check PA.Formula.rename_positiveCommonMultipleThroughTermAt.
 Check PA.Formula.subst_betaCodingStepTermAt.
@@ -225,6 +229,12 @@ Check PA.Formula.subst_betaPrependCodingStepTermAt.
 Check PA.Formula.rename_betaPrependCodingStepTermAt.
 Check PA.Formula.subst_betaPrependCodingStepExistsTermAt.
 Check PA.Formula.rename_betaPrependCodingStepExistsTermAt.
+Check PA.Formula.subst_betaUnshiftPrefixTermAt.
+Check PA.Formula.rename_betaUnshiftPrefixTermAt.
+Check PA.Formula.subst_betaPrependPrefixTermAt.
+Check PA.Formula.rename_betaPrependPrefixTermAt.
+Check PA.Formula.subst_betaPrependPrefixCodeExistsTermAt.
+Check PA.Formula.rename_betaPrependPrefixCodeExistsTermAt.
 Check PA.Formula.positiveCommonMultipleExistsTermAt.
 Check PA.Formula.positiveCommonMultipleExistsTermAtBody.
 Check PA.Formula.subst_positiveCommonMultipleExistsTermAt.
